\subsection{Definitions}
\begin{align*}
b&=\sqrt{a} : b \geq 0 \wedge b^2=a \\
\sqrt{a^2}&= \vert a \vert \\
\text{If } a&\geq \text{ then } \sqrt{a^2}=a
\end{align*}
\subsection{Distributing}
$(a\geq 0 \wedge b\geq 0)$
\begin{align*}
\sqrt{ab}&=\sqrt{a}\sqrt{b} \\
\sqrt{\frac{a}{b}}&= \frac{\sqrt{a}}{\sqrt{b}}\qquad(b\neq 0) \\
\sqrt{a}\sqrt{a}&=a\\
\sqrt{a^n}&=\left( \sqrt{a} \right) ^n \vee a^{\frac{n}{2}}
\end{align*}
\subsection{Rationalizing the Denominator}
$(a>0 \wedge b>0 \wedge c>0)$
\begin{align*}
\frac{a}{\sqrt{b}}=\frac{a}{\sqrt{b}}\cdot\frac{\sqrt{b}}{\sqrt{b}}&=\frac{a\sqrt{b}}{b} 
&
\frac{4}{\sqrt{2}}=\frac{4}{\sqrt{2}}\cdot\frac{\sqrt{2}}{\sqrt{2}}&=\frac{4\sqrt{2}}{2}=2\sqrt{2} \\ \\
\frac{a}{b+\sqrt{c}}=\frac{a}{b+\sqrt{c}}\cdot \frac{b-\sqrt{c}}{b-\sqrt{c}}&=\frac{ab-a\sqrt{c}}{b^2-c}
&
\frac{6}{3+\sqrt{7}}=\frac{6}{3+\sqrt{7}}\cdot\frac{3-\sqrt{7}}{3-\sqrt{7}}&=\frac{18-6\sqrt{7}}{9-7} \\
& & = \frac{18-6\sqrt{7}}{9-7}=\frac{18-6\sqrt{7}}{2}&=9-3\sqrt{7} \\ \\
\frac{a}{b-\sqrt{c}}=\frac{a}{b-\sqrt{c}} \cdot \frac{b+\sqrt{c}}{b+\sqrt{c}} &= \frac{ab+a\sqrt{c}}{b^2-c}
&
\frac{5}{2-\sqrt{3}}=\frac{5}{2-\sqrt{3}}\cdot\frac{2+\sqrt{3}}{2+\sqrt{3}}&=\frac{10+5\sqrt{3}}{4-3} \\
& & =\frac{10+5\sqrt{3}}{1}&=10+5\sqrt{3} \\ \\
\frac{a}{\sqrt{b}+\sqrt{c}}=\frac{a}{\sqrt{b}+\sqrt{c}}\cdot \frac{\sqrt{b}-\sqrt{c}}{\sqrt{b}-\sqrt{c}}&=\frac{a\sqrt{b}-a\sqrt{c}}{b-c}
&
\frac{14}{\sqrt{13}+\sqrt{11}}=\frac{14}{\sqrt{13}+\sqrt{11}}\cdot \frac{\sqrt{13}-\sqrt{11}}{\sqrt{13}-\sqrt{11}}&=\frac{14\sqrt{13}-14\sqrt{11}}{13-11}\\
& & = \frac{14\sqrt{13}-14\sqrt{11}}{2}&=7\sqrt{13}-7\sqrt{11} \\ \\
\frac{a}{\sqrt{b}-\sqrt{c}}=\frac{a}{\sqrt{b}-\sqrt{c}}\cdot \frac{\sqrt{b}+\sqrt{c}}{\sqrt{b}+\sqrt{c}}&=\frac{a\sqrt{b}+a\sqrt{c}}{b-c}
&
\frac{12}{\sqrt{15}-\sqrt{7}}=\frac{12}{\sqrt{15}-\sqrt{7}} \cdot \frac{\sqrt{15}+\sqrt{7}}{\sqrt{15}+\sqrt{7}}&=\frac{12\sqrt{15}+12\sqrt{7}}{15-7}\\
& & = \frac{12\sqrt{15}+12\sqrt{7}}{8}&=\frac{3\sqrt{15}+2\sqrt{7}}{2}
\end{align*}
\subsection{OBS!}
\begin{align*}
\sqrt{a+b}&\neq \sqrt{a}+\sqrt{b}\\
\sqrt{a-b}&\neq \sqrt{a}-\sqrt{b}\\
\sqrt{a^2+b^2}&\neq a+b
\end{align*}
